lakefile.lean
@@ -3,8 +3,6 @@ open Lake DSL
 
 package «mm-lean4»
 
-require std from git "https://github.com/leanprover/std4" @ "main"
-
 @[default_target]
 lean_lib Metamath where
   roots := #[`Metamath.Verify]
